theories/ExamplesUtil.v
@@ -5,39 +5,12 @@ From Equations Require Import Equations DepElimDec.
 From Template Require Import utils Ast LiftSubst Typing Checker.
 From Translation Require Import util Quotes Sorts SAst SLiftSubst SCommon
      ITyping ITypingInversions ITypingLemmata ITypingAdmissible XTyping
-     FundamentalLemma Translation FinalTranslation FullQuote.
+     FundamentalLemma Translation FinalTranslation FullQuote ExampleQuotes.
 
 (* For efficiency reasons we use type in type for examples. *)
 Existing Instance Sorts.type_in_type.
 
 (* The context for Template Coq *)
-
-Inductive vec A : nat -> Type :=
-| vnil : vec A 0
-| vcons : A -> forall n, vec A n -> vec A (S n).
-
-Arguments vnil {_}.
-Arguments vcons {_} _ _ _.
-
-(* Definition axiom_nat_ty := ltac:(let t := type of axiom_nat in exact t). *)
-(* Definition axiom_zero_ty := ltac:(let t := type of axiom_zero in exact t). *)
-(* Definition axiom_succ_ty := ltac:(let t := type of axiom_succ in exact t). *)
-(* Definition axiom_nat_rect_ty := *)
-(*   ltac:(let t := type of axiom_nat_rect in exact t). *)
-(* Definition axiom_nat_rect_zero_ty := *)
-(*   ltac:(let t := type of axiom_nat_rect_zero in exact t). *)
-(* Definition axiom_nat_rect_succ_ty := *)
-(*   ltac:(let t := type of axiom_nat_rect_succ in exact t). *)
-
-(* Definition axiom_vec_ty := ltac:(let t := type of axiom_vec in exact t). *)
-(* Definition axiom_vnil_ty := ltac:(let t := type of axiom_vnil in exact t). *)
-(* Definition axiom_vcons_ty := ltac:(let t := type of axiom_vcons in exact t). *)
-(* Definition axiom_vec_rect_ty := *)
-(*   ltac:(let t := type of axiom_vec_rect in exact t). *)
-(* Definition axiom_vec_rect_vnil_ty := *)
-(*   ltac:(let t := type of axiom_vec_rect_vnil in exact t). *)
-(* Definition axiom_vec_rect_vcons_ty := *)
-(*   ltac:(let t := type of axiom_vec_rect_vcons in exact t). *)
 
 (* We define a term that mentions everything that the global context should
    have. *)
@@ -71,32 +44,6 @@ Definition glob_term :=
   let _ := @cong_refl in
   let _ := @eq_to_heq in
   let _ := @heq_type_eq in
-  (* Axiomatising nat *)
-  (* let _ := @axiom_nat in *)
-  (* let _ := @axiom_nat_ty in *)
-  (* let _ := @axiom_zero in *)
-  (* let _ := @axiom_zero_ty in *)
-  (* let _ := @axiom_succ in *)
-  (* let _ := @axiom_succ_ty in *)
-  (* let _ := @axiom_nat_rect in *)
-  (* let _ := @axiom_nat_rect_ty in *)
-  (* let _ := @axiom_nat_rect_zero in *)
-  (* let _ := @axiom_nat_rect_zero_ty in *)
-  (* let _ := @axiom_nat_rect_succ in *)
-  (* let _ := @axiom_nat_rect_succ_ty in *)
-  (* Vec *)
-  (* let _ := @axiom_vec in *)
-  (* let _ := @axiom_vnil in *)
-  (* let _ := @axiom_vcons in *)
-  (* let _ := @axiom_vec_rect in *)
-  (* let _ := @axiom_vec_rect_vnil in *)
-  (* let _ := @axiom_vec_rect_vcons in *)
-  (* let _ := @axiom_vec_ty in *)
-  (* let _ := @axiom_vnil_ty in *)
-  (* let _ := @axiom_vcons_ty in *)
-  (* let _ := @axiom_vec_rect_ty in *)
-  (* let _ := @axiom_vec_rect_vnil_ty in *)
-  (* let _ := @axiom_vec_rect_vcons_ty in *)
   (* Candidate *)
   let _ := @candidate in
   (* For examples *)
@@ -104,14 +51,15 @@ Definition glob_term :=
   let _ := vec in
   let _ := vec_rect in
   let _ := Nat.add in
+  let _ := vrev_eq0 in
+  let _ := vrev_eq1 in
   Type.
 
 Quote Recursively Definition glob_prog := @glob_term.
 Definition Σ : global_context :=
+  (* Eval lazy in *)
   (* reconstruct_global_context (Datatypes.fst glob_prog). *)
   pair (Datatypes.fst glob_prog) init_graph.
-
-(* Definition Σ := ltac:(let t := eval lazy in Σ' in exact t). *)
 
 Arguments Σ : simpl never.
 
@@ -289,262 +237,157 @@ Ltac ittcheck' := ittcheck1 ; try (lazy ; omega).
 
 Ltac ittcheck := repeat ittcheck'.
 
-(* Getting axiom_nat as an axiom for ITT/ETT *)
-(* Quote Recursively Definition taxiom_nat_ty := axiom_nat_ty. *)
-(* Definition ttaxiom_nat_ty := *)
-(*   let t := Datatypes.snd taxiom_nat_ty in *)
-(*   match hnf Σ [] t with *)
-(*   | Checked t => t *)
-(*   | _ => tRel 0 *)
-(*   end. *)
-(* Definition rtaxiom_nat_ty := *)
-(*   ltac:(let u := eval lazy in ttaxiom_nat_ty in exact u). *)
+(* Preparing the global context (axioms) for examples *)
 
-(* Definition fq_ax_nat_ty := *)
-(*   fullquote (2 ^ 18) Σ [] rtaxiom_nat_ty. *)
-(* Definition rfq_ax_nat_ty := *)
-(*   ltac:(let u := eval lazy in fq_ax_nat_ty in exact u). *)
-(* Definition ax_nat_ty := *)
-(*   match rfq_ax_nat_ty with *)
-(*   | Success t => t *)
-(*   | _ => sRel 0 *)
-(*   end. *)
-(* Definition rtax_nat_ty := *)
-(*   ltac:(let u := eval lazy in ax_nat_ty in exact u). *)
+Notation "s --> t" := (acons s t) (at level 20).
+Notation "[< a ; b ; .. ; c >]" :=
+  (a (b (.. (c empty) ..))).
+Notation "[< a >]" := (a empty).
+Notation "[< >]" := (empty).
 
-(* Getting axiom_nat_rect as an axiom for ITT/ETT *)
-(* Quote Recursively Definition taxiom_nat_rect_ty := axiom_nat_rect_ty. *)
-(* Definition ttaxiom_nat_rect_ty := *)
-(*   let t := Datatypes.snd taxiom_nat_rect_ty in *)
-(*   match hnf Σ [] t with *)
-(*   | Checked t => t *)
-(*   | _ => tRel 0 *)
-(*   end. *)
-(* Definition rtaxiom_nat_rect_ty := *)
-(*   ltac:(let u := eval lazy in ttaxiom_nat_rect_ty in exact u). *)
+(* Notation "[< a --> x ; b --> y ; .. ; c --> z >]" := *)
+(*   (acons a x (acons b y .. (acons c z empty) ..)). *)
 
-(* Definition fq_ax_nat_rect_ty := *)
-(*   fullquote (2 ^ 18) Σ [] rtaxiom_nat_rect_ty. *)
-(* Definition rfq_ax_nat_rect_ty := *)
-(*   ltac:(let u := eval lazy in fq_ax_nat_rect_ty in exact u). *)
-(* Definition ax_nat_rect_ty := *)
-(*   match rfq_ax_nat_rect_ty with *)
-(*   | Success t => t *)
-(*   | _ => sRel 0 *)
-(*   end. *)
-(* Definition rtax_nat_rect_ty := *)
-(*   ltac:(let u := eval lazy in ax_nat_rect_ty in exact u). *)
+Definition indt :=
+  [< "Coq.Init.Datatypes.nat" --> sAx "nat" ;
+     "Translation.ExampleQuotes.vec" --> sAx "vec"
+  >].
 
+Definition constt :=
+  [< "Coq.Init.Nat.add" --> sAx "add" ;
+     "Translation.ExampleQuotes.vec_rect" --> sAx "vec_rect"
+  >].
 
+Definition cot (id : string) (n : nat) : option sterm :=
+  match id, n with
+  | "Coq.Init.Datatypes.nat", 0 => Some (sAx "O")
+  | "Coq.Init.Datatypes.nat", 1 => Some (sAx "S")
+  | "Translation.ExampleQuotes.vec", 0 => Some (sAx "vnil")
+  | "Translation.ExampleQuotes.vec", 1 => Some (sAx "vcons")
+  | _,_ => None
+  end.
 
-(* axiom_nat_rect_zero *)
-(* Quote Recursively Definition taxiom_nat_rect_zero_ty := axiom_nat_rect_zero_ty. *)
-(* Definition ttaxiom_nat_rect_zero_ty := *)
-(*   let t := Datatypes.snd taxiom_nat_rect_zero_ty in *)
-(*   match hnf Σ [] t with *)
-(*   | Checked t => t *)
-(*   | _ => tRel 0 *)
-(*   end. *)
-(* Definition rtaxiom_nat_rect_zero_ty := *)
-(*   ltac:(let u := eval lazy in ttaxiom_nat_rect_zero_ty in exact u). *)
-(* Definition fq_ax_nat_rect_zero_ty := *)
-(*   fullquote (2 ^ 18) Σ [] rtaxiom_nat_rect_zero_ty. *)
-(* Definition rfq_ax_nat_rect_zero_ty := *)
-(*   ltac:(let u := eval lazy in fq_ax_nat_rect_zero_ty in exact u). *)
-(* Definition ax_nat_rect_zero_ty := *)
-(*   match rfq_ax_nat_rect_zero_ty with *)
-(*   | Success t => t *)
-(*   | _ => sRel 0 *)
-(*   end. *)
-(* Definition rtax_nat_rect_zero_ty := *)
-(*   ltac:(let u := eval lazy in ax_nat_rect_zero_ty in exact u). *)
+(* nat *)
+Quote Definition nat_type := 
+  ltac:(let T := type of nat in exact T).
+Definition prety_nat :=
+  Eval lazy in fullquote (2 ^ 18) Σ [] nat_type indt constt cot.
+Definition ty_nat :=
+  Eval lazy in 
+  match prety_nat with
+  | Success t => t
+  | Error _ => sRel 0
+  end.
 
+(* O *)
+Quote Definition O_type := 
+  ltac:(let T := type of O in exact T).
+Definition prety_O :=
+  Eval lazy in fullquote (2 ^ 18) Σ [] O_type indt constt cot.
+Definition ty_O :=
+  Eval lazy in 
+  match prety_O with
+  | Success t => t
+  | Error _ => sRel 0
+  end.
 
+(* S *)
+Quote Definition S_type := 
+  ltac:(let T := type of S in exact T).
+Definition prety_S :=
+  Eval lazy in fullquote (2 ^ 18) Σ [] S_type indt constt cot.
+Definition ty_S :=
+  Eval lazy in 
+  match prety_S with
+  | Success t => t
+  | Error _ => sRel 0
+  end.
 
-(* axiom_nat_rect_succ *)
-(* Quote Recursively Definition taxiom_nat_rect_succ_ty := axiom_nat_rect_succ_ty. *)
-(* Definition ttaxiom_nat_rect_succ_ty := *)
-(*   let t := Datatypes.snd taxiom_nat_rect_succ_ty in *)
-(*   match hnf Σ [] t with *)
-(*   | Checked t => t *)
-(*   | _ => tRel 0 *)
-(*   end. *)
-(* Definition rtaxiom_nat_rect_succ_ty := *)
-(*   ltac:(let u := eval lazy in ttaxiom_nat_rect_succ_ty in exact u). *)
-(* Definition fq_ax_nat_rect_succ_ty := *)
-(*   fullquote (2 ^ 18) Σ [] rtaxiom_nat_rect_succ_ty. *)
-(* Definition rfq_ax_nat_rect_succ_ty := *)
-(*   ltac:(let u := eval lazy in fq_ax_nat_rect_succ_ty in exact u). *)
-(* Definition ax_nat_rect_succ_ty := *)
-(*   match rfq_ax_nat_rect_succ_ty with *)
-(*   | Success t => t *)
-(*   | _ => sRel 0 *)
-(*   end. *)
-(* Definition rtax_nat_rect_succ_ty := *)
-(*   ltac:(let u := eval lazy in ax_nat_rect_succ_ty in exact u). *)
+(* vec *)
+Quote Definition vec_type := 
+  ltac:(let T := type of vec in exact T).
+Definition prety_vec :=
+  Eval lazy in fullquote (2 ^ 18) Σ [] vec_type indt constt cot.
+Definition ty_vec :=
+  Eval lazy in 
+  match prety_vec with
+  | Success t => t
+  | Error _ => sRel 0
+  end.
 
+(* vnil *)
+Quote Definition vnil_type :=
+  ltac:(let T := type of @vnil in exact T).
+Definition prety_vnil :=
+  Eval lazy in fullquote (2 ^ 18) Σ [] vnil_type indt constt cot.
+Definition ty_vnil :=
+  Eval lazy in
+  match prety_vnil with
+  | Success t => t
+  | Error _ => sRel 0
+  end.
 
+(* vcons *)
+Quote Definition vcons_type :=
+  ltac:(let T := type of @vcons in exact T).
+Definition prety_vcons :=
+  Eval lazy in fullquote (2 ^ 18) Σ [] vcons_type indt constt cot.
+Definition ty_vcons :=
+  Eval lazy in
+  match prety_vcons with
+  | Success t => t
+  | Error _ => sRel 0
+  end.
 
-(* axiom_vec *)
-(* Quote Recursively Definition taxiom_vec_ty := axiom_vec_ty. *)
-(* Definition ttaxiom_vec_ty := *)
-(*   let t := Datatypes.snd taxiom_vec_ty in *)
-(*   match hnf Σ [] t with *)
-(*   | Checked t => t *)
-(*   | _ => tRel 0 *)
-(*   end. *)
-(* Definition rtaxiom_vec_ty := *)
-(*   ltac:(let u := eval lazy in ttaxiom_vec_ty in exact u). *)
-(* Definition fq_ax_vec_ty := *)
-(*   fullquote (2 ^ 18) Σ [] rtaxiom_vec_ty. *)
-(* Definition rfq_ax_vec_ty := *)
-(*   ltac:(let u := eval lazy in fq_ax_vec_ty in exact u). *)
-(* Definition ax_vec_ty := *)
-(*   match rfq_ax_vec_ty with *)
-(*   | Success t => t *)
-(*   | _ => sRel 0 *)
-(*   end. *)
-(* Definition rtax_vec_ty := *)
-(*   ltac:(let u := eval lazy in ax_vec_ty in exact u). *)
+(* add *)
+Quote Definition add_type :=
+  ltac:(let T := type of @Nat.add in exact T).
+Definition prety_add :=
+  Eval lazy in fullquote (2 ^ 18) Σ [] add_type indt constt cot.
+Definition ty_add :=
+  Eval lazy in
+  match prety_add with
+  | Success t => t
+  | Error _ => sRel 0
+  end.
 
+(* vrev_eq0 *)
+Quote Definition vrev_eq0_type :=
+  ltac:(let T := type of @vrev_eq0 in exact T).
+Definition prety_vrev_eq0 :=
+  Eval lazy in fullquote (2 ^ 18) Σ [] vrev_eq0_type indt constt cot.
+Definition ty_vrev_eq0 :=
+  Eval lazy in
+  match prety_vrev_eq0 with
+  | Success t => t
+  | Error _ => sRel 0
+  end.
 
-
-(* axiom_vnil *)
-(* Quote Recursively Definition taxiom_vnil_ty := axiom_vnil_ty. *)
-(* Definition ttaxiom_vnil_ty := *)
-(*   let t := Datatypes.snd taxiom_vnil_ty in *)
-(*   match hnf Σ [] t with *)
-(*   | Checked t => t *)
-(*   | _ => tRel 0 *)
-(*   end. *)
-(* Definition rtaxiom_vnil_ty := *)
-(*   ltac:(let u := eval lazy in ttaxiom_vnil_ty in exact u). *)
-(* Definition fq_ax_vnil_ty := *)
-(*   fullquote (2 ^ 18) Σ [] rtaxiom_vnil_ty. *)
-(* Definition rfq_ax_vnil_ty := *)
-(*   ltac:(let u := eval lazy in fq_ax_vnil_ty in exact u). *)
-(* Definition ax_vnil_ty := *)
-(*   match rfq_ax_vnil_ty with *)
-(*   | Success t => t *)
-(*   | _ => sRel 0 *)
-(*   end. *)
-(* Definition rtax_vnil_ty := *)
-(*   ltac:(let u := eval lazy in ax_vnil_ty in exact u). *)
-
-
-
-(* axiom_vcons *)
-(* Quote Recursively Definition taxiom_vcons_ty := axiom_vcons_ty. *)
-(* Definition ttaxiom_vcons_ty := *)
-(*   let t := Datatypes.snd taxiom_vcons_ty in *)
-(*   match hnf Σ [] t with *)
-(*   | Checked t => t *)
-(*   | _ => tRel 0 *)
-(*   end. *)
-(* Definition rtaxiom_vcons_ty := *)
-(*   ltac:(let u := eval lazy in ttaxiom_vcons_ty in exact u). *)
-(* Definition fq_ax_vcons_ty := *)
-(*   fullquote (2 ^ 18) Σ [] rtaxiom_vcons_ty. *)
-(* Definition rfq_ax_vcons_ty := *)
-(*   ltac:(let u := eval lazy in fq_ax_vcons_ty in exact u). *)
-(* Definition ax_vcons_ty := *)
-(*   match rfq_ax_vcons_ty with *)
-(*   | Success t => t *)
-(*   | _ => sRel 0 *)
-(*   end. *)
-(* Definition rtax_vcons_ty := *)
-(*   ltac:(let u := eval lazy in ax_vcons_ty in exact u). *)
-
-
-
-(* axiom_vec_rect *)
-(* Quote Recursively Definition taxiom_vec_rect_ty := axiom_vec_rect_ty. *)
-(* Definition ttaxiom_vec_rect_ty := *)
-(*   let t := Datatypes.snd taxiom_vec_rect_ty in *)
-(*   match hnf Σ [] t with *)
-(*   | Checked t => t *)
-(*   | _ => tRel 0 *)
-(*   end. *)
-(* Definition rtaxiom_vec_rect_ty := *)
-(*   ltac:(let u := eval lazy in ttaxiom_vec_rect_ty in exact u). *)
-(* Definition fq_ax_vec_rect_ty := *)
-(*   fullquote (2 ^ 18) Σ [] rtaxiom_vec_rect_ty. *)
-(* Definition rfq_ax_vec_rect_ty := *)
-(*   ltac:(let u := eval lazy in fq_ax_vec_rect_ty in exact u). *)
-(* Definition ax_vec_rect_ty := *)
-(*   match rfq_ax_vec_rect_ty with *)
-(*   | Success t => t *)
-(*   | _ => sRel 0 *)
-(*   end. *)
-(* Definition rtax_vec_rect_ty := *)
-(*   ltac:(let u := eval lazy in ax_vec_rect_ty in exact u). *)
-
-
-
-(* axiom_vec_rect_vnil *)
-(* Quote Recursively Definition taxiom_vec_rect_vnil_ty := axiom_vec_rect_vnil_ty. *)
-(* Definition ttaxiom_vec_rect_vnil_ty := *)
-(*   let t := Datatypes.snd taxiom_vec_rect_vnil_ty in *)
-(*   match hnf Σ [] t with *)
-(*   | Checked t => t *)
-(*   | _ => tRel 0 *)
-(*   end. *)
-(* Definition rtaxiom_vec_rect_vnil_ty := *)
-(*   ltac:(let u := eval lazy in ttaxiom_vec_rect_vnil_ty in exact u). *)
-(* Definition fq_ax_vec_rect_vnil_ty := *)
-(*   fullquote (2 ^ 18) Σ [] rtaxiom_vec_rect_vnil_ty. *)
-(* Definition rfq_ax_vec_rect_vnil_ty := *)
-(*   ltac:(let u := eval lazy in fq_ax_vec_rect_vnil_ty in exact u). *)
-(* Definition ax_vec_rect_vnil_ty := *)
-(*   match rfq_ax_vec_rect_vnil_ty with *)
-(*   | Success t => t *)
-(*   | _ => sRel 0 *)
-(*   end. *)
-(* Definition rtax_vec_rect_vnil_ty := *)
-(*   ltac:(let u := eval lazy in ax_vec_rect_vnil_ty in exact u). *)
-
-
-
-(* axiom_vec_rect_vcons *)
-(* Quote Recursively Definition taxiom_vec_rect_vcons_ty := axiom_vec_rect_vcons_ty. *)
-(* Definition ttaxiom_vec_rect_vcons_ty := *)
-(*   let t := Datatypes.snd taxiom_vec_rect_vcons_ty in *)
-(*   match hnf Σ [] t with *)
-(*   | Checked t => t *)
-(*   | _ => tRel 0 *)
-(*   end. *)
-(* Definition rtaxiom_vec_rect_vcons_ty := *)
-(*   ltac:(let u := eval lazy in ttaxiom_vec_rect_vcons_ty in exact u). *)
-(* Definition fq_ax_vec_rect_vcons_ty := *)
-(*   fullquote (2 ^ 18) Σ [] rtaxiom_vec_rect_vcons_ty. *)
-(* Definition rfq_ax_vec_rect_vcons_ty := *)
-(*   ltac:(let u := eval lazy in fq_ax_vec_rect_vcons_ty in exact u). *)
-(* Definition ax_vec_rect_vcons_ty := *)
-(*   match rfq_ax_vec_rect_vcons_ty with *)
-(*   | Success t => t *)
-(*   | _ => sRel 0 *)
-(*   end. *)
-(* Definition rtax_vec_rect_vcons_ty := *)
-(*   ltac:(let u := eval lazy in ax_vec_rect_vcons_ty in exact u). *)
-
-
+(* vrev_eq1 *)
+Quote Definition vrev_eq1_type :=
+  ltac:(let T := type of @vrev_eq1 in exact T).
+Definition prety_vrev_eq1 :=
+  Eval lazy in fullquote (2 ^ 18) Σ [] vrev_eq1_type indt constt cot.
+Definition ty_vrev_eq1 :=
+  Eval lazy in
+  match prety_vrev_eq1 with
+  | Success t => t
+  | Error _ => sRel 0
+  end.
 
 
 (* The global context *)
 
 Definition Σi : sglobal_context := [
-  (* decl "vec_rect_vcons" rtax_vec_rect_vcons_ty ; *)
-  (* decl "vec_rect_vnil" rtax_vec_rect_vnil_ty ; *)
-  (* decl "vec_rect" rtax_vec_rect_ty ; *)
-  (* decl "vcons" rtax_vcons_ty ; *)
-  (* decl "vnil" rtax_vnil_ty ; *)
-  (* decl "vec" rtax_vec_ty ; *)
-  (* decl "nat_rect_succ" rtax_nat_rect_succ_ty ; *)
-  (* decl "nat_rect_zero" rtax_nat_rect_zero_ty ; *)
-  (* decl "nat_rect" rtax_nat_rect_ty ; *)
-  (* decl "succ" (sAx "nat" ==> sAx "nat") ; *)
-  (* decl "zero" (sAx "nat") ; *)
-  (* decl "nat" rtax_nat_ty *)
+  decl "vrev_eq1" ty_vrev_eq1 ;
+  decl "vrev_eq0" ty_vrev_eq0 ;
+  decl "add" ty_add ;
+  decl "vcons" ty_vcons ;
+  decl "vnil" ty_vnil ;
+  decl "vec" ty_vec ;
+  decl "S" ty_S ;
+  decl "O" ty_O ;
+  decl "nat" ty_nat
 ].
 
 Arguments Σi : simpl never.
@@ -552,18 +395,15 @@ Arguments Σi : simpl never.
 Fact hΣi : type_glob Σi.
 Proof.
   repeat glob ; lazy.
-  (* - ittcheck. *)
-  (* - ittcheck. *)
-  (* - ittcheck. *)
-  (* - ittcheck. *)
-  (* - ittcheck. *)
-  (* - ittcheck. *)
-  (* - ittcheck. *)
-  (* - ittcheck. *)
-  (* - ittcheck. *)
-  (* - ittcheck. *)
-  (* - ittcheck. *)
-  (* - ittcheck. *)
+  - ittcheck.
+  - ittcheck.
+  - ittcheck.
+  - ittcheck.
+  - ittcheck.
+  - ittcheck.
+  - ittcheck.
+  - ittcheck.
+  - ittcheck.
 Defined.
 
 (* Now some useful lemmata *)
