theories/ExampleQuotes.v
@@ -1,0 +1,23 @@
+(* Quotations of terms for examples *)
+
+From Coq Require Import Bool String List BinPos Compare_dec Omega.
+From Equations Require Import Equations DepElimDec.
+From Template Require Import Ast LiftSubst Typing Checker.
+From Translation Require Import util.
+
+Inductive vec A : nat -> Type :=
+| vnil : vec A 0
+| vcons : A -> forall n, vec A n -> vec A (S n).
+
+Arguments vnil {_}.
+Arguments vcons {_} _ _ _.
+
+Lemma vrev_eq0 : forall A m, vec A (0 + m) = vec A m.
+Proof.
+  reflexivity.
+Defined.
+
+Lemma vrev_eq1 : forall A n m, vec A (n + S m) = vec A (S n + m).
+Proof.
+  intros A n m. f_equal. omega.
+Defined.
